feat: synthetic_main_lemma

src/QL/FOL/Tait/calculus.lean
@@ -1,4 +1,4 @@
-import QL.FOL.Tait.tait QL.FOL.semantics QL.FOL.language logic
+import QL.FOL.Tait.tait QL.FOL.semantics QL.FOL.Tait.coding logic
 
 universes u v
 
@@ -10,7 +10,7 @@ namespace Tait
 variables {L : language.{u}} {m n : ℕ}
 namespace subformula
 
-variables (S : Structure L) {m n} {me : fin m → S} {e : fin n → S}
+variables (S : Structure L) {n} {me : fin m → S} {e : fin n → S}
 
 @[simp] def val' (me : fin m → S) : ∀ {n} (e : fin n → S), subformula L m n → Prop
 | n _ verum              := true
@@ -57,11 +57,9 @@ end formula
 
 def models (S : Structure L) (p : formula L m) : Prop := ∀ e, formula.val S e p
 
-
 namespace sentence
 variables (S : Structure L)
 
-def models : sentence L →ₗ Prop := subformula.val S fin.nil fin.nil  
 
 end sentence
 
@@ -70,44 +68,112 @@ open subformula
 noncomputable def finset_mlift (Δ : finset (subformula L m n)) : finset (subformula L (m + 1) n) := Δ.image mlift
 
 -- Tate caluculus
-inductive derivative : Π {m}, finset (subformula L m 0) → Type u
-| AxL {m} : ∀ (Δ : finset (subformula L m 0)) {k} (r : L.pr k) (v : fin k → subterm L m 0),
+inductive derivative : Π {m}, finset (formula L m) → Type u
+| AxL {m} : ∀ (Δ : finset (formula L m)) {k} (r : L.pr k) (v : fin k → subterm L m 0),
     relation r v ∈ Δ → neg_relation r v ∈ Δ → derivative Δ
-| or_left {m} : ∀ (Δ : finset (subformula L m 0)) (p q : formula L m),
+| verum {m} : ∀ (Δ : finset (formula L m)), ⊤ ∈ Δ → derivative Δ
+| or_left {m} : ∀ (Δ : finset (formula L m)) (p q : formula L m),
     derivative (insert p Δ) → derivative (insert (p ⊔ q) Δ)
-| or_right {m} : ∀ (Δ : finset (subformula L m 0)) (p q : formula L m),
+| or_right {m} : ∀ (Δ : finset (formula L m)) (p q : formula L m),
     derivative (insert q Δ) → derivative (insert (p ⊔ q) Δ)
-| and {m} : ∀ (Δ : finset (subformula L m 0)) (p q : formula L m),
+| and {m} : ∀ (Δ : finset (formula L m)) (p q : formula L m),
     derivative (insert p Δ) → derivative (insert q Δ) → derivative (insert (p ⊓ q) Δ)
 | all {m} : ∀ (Δ : finset (subformula L m 0)) (p : subformula L m 1),
     derivative (insert p.push (finset_mlift Δ)) → derivative (insert (∀'p) Δ)
-| ex {m} : ∀ (Δ : finset (subformula L m 0)) (t) (p : subformula L m 1),
+| ex {m} : ∀ (Δ : finset (subformula L m 0)) (t : subterm L m 0) (p : subformula L m 1),
     derivative (insert (subst t p) Δ) → derivative (insert (∃'p) Δ)
 
-variables {Δ : finset (subformula L m 0)}
-open axiomatic_classical_logic' axiomatic_classical_logic
+variables {L m}
 
-prefix `⊢ᵀ `:45 := derivative
+def derivable {m} (Δ : finset (formula L m)) : Prop := nonempty (derivative Δ)
 
-open language
+prefix `⊢ᵀ `:45 := derivable
 
-def add_nat (L : language) := L.padd (Constants ℕ)
-#check @padd_left
-def uniformal_genelization (Γ : finset (subformula (add_nat L) m 0)) (Δ : finset (subformula L m 0)) (p : subformula L m 1) (c) :
-  ⊢ᵀ Γ → Γ = insert (subst c $ of_lhom (@padd_left L (Constants ℕ)) p) (Δ.image $ of_lhom (@padd_left L (Constants ℕ))) →
-  ⊢ᵀ insert p.push (finset_mlift Δ) := λ h,
+namespace derivable
+variables {m} {Δ Γ : finset (formula L m)}
+
+lemma AxL {k} (r : L.pr k) (v : fin k → subterm L m 0) (h : relation r v ∈ Δ) (hneg : neg_relation r v ∈ Δ) : ⊢ᵀ Δ :=
+⟨derivative.AxL Δ r v h hneg⟩
+
+lemma verum (h : ⊤ ∈ Δ) : ⊢ᵀ Δ := ⟨derivative.verum Δ h⟩
+
+lemma or_left (p q : formula L m) : ⊢ᵀ insert p Δ → ⊢ᵀ insert (p ⊔ q) Δ := λ ⟨d⟩, ⟨derivative.or_left Δ p q d⟩
+
+lemma or_right (p q : formula L m) : ⊢ᵀ insert q Δ → ⊢ᵀ insert (p ⊔ q) Δ := λ ⟨d⟩, ⟨derivative.or_right Δ p q d⟩
+
+lemma and (p q : formula L m) : ⊢ᵀ insert p Δ → ⊢ᵀ insert q Δ → ⊢ᵀ insert (p ⊓ q) Δ := λ ⟨d₁⟩ ⟨d₂⟩, ⟨derivative.and Δ p q d₁ d₂⟩
+
+lemma all (p : subformula L m 1) : ⊢ᵀ insert p.push (finset_mlift Δ) → ⊢ᵀ insert (∀'p) Δ := λ ⟨d⟩, ⟨derivative.all Δ p d⟩
+
+lemma ex (t) (p : subformula L m 1) : ⊢ᵀ insert (subst t p) Δ → ⊢ᵀ insert (∃'p) Δ := λ ⟨d⟩, ⟨derivative.ex Δ t p d⟩
+
+protected lemma cast (h : ⊢ᵀ Δ) (e : Δ = Γ) : ⊢ᵀ Γ := cast (by rw e) h
+
+@[elab_as_eliminator]
+theorem rec_on {C : Π {m} (Δ : finset (formula L m)), ⊢ᵀ Δ → Prop}
+  {m : ℕ} {Δ : finset (formula L m)} (d : ⊢ᵀ Δ)
+  (hAxL : ∀ {m} (Δ : finset (formula L m)) {k} (r : L.pr k) (v : fin k → subterm L m 0)
+    (h : relation r v ∈ Δ) (hneg : neg_relation r v ∈ Δ), C Δ (AxL r v h hneg))
+  (hverum : ∀ {m} (Δ : finset (formula L m)) (h : ⊤ ∈ Δ), C Δ (verum h))
+  (hor_left : ∀ {m} (Δ : finset (formula L m)) (p q : formula L m) (d : ⊢ᵀ insert p Δ),
+    C (insert p Δ) d → C (insert (p ⊔ q) Δ) (or_left p q d))
+  (hor_right : ∀ {m} (Δ : finset (formula L m)) (p q : formula L m) (d : ⊢ᵀ insert q Δ),
+    C (insert q Δ) d → C (insert (p ⊔ q) Δ) (or_right p q d))
+  (hand : ∀ {m} (Δ : finset (formula L m)) (p q : formula L m) (d₁ : ⊢ᵀ insert p Δ) (d₂ : ⊢ᵀ insert q Δ),
+    C (insert p Δ) d₁ → C (insert q Δ) d₂ → C (insert (p ⊓ q) Δ) (and p q d₁ d₂))
+  (hall : ∀ {m} (Δ : finset (formula L m)) (p : subformula L m 1) (d : ⊢ᵀ insert p.push (finset_mlift Δ)),
+    C (insert p.push (finset_mlift Δ)) d → C (insert (∀'p) Δ) (all p d))
+  (hex : ∀ {m} (Δ : finset (formula L m)) (t) (p : subformula L m 1) (d : ⊢ᵀ insert (subst t p) Δ),
+    C (insert (subst t p) Δ) d → C (insert (∃'p) Δ) (ex t p d)) : C Δ d :=
+ by unfreezingI {
+  begin
+    cases d,
+    induction d,
+    case AxL : m Δ k r v h hneg { exact hAxL Δ r v h hneg },
+    case verum : m Δ h { exact hverum Δ h },
+    case or_left : m Δ p q _ ih { exact hor_left Δ p q _ ih },
+    case or_right : m Δ p q _ ih { exact hor_right Δ p q _ ih },
+    case and : m Δ p q _ _ ih₁ ih₂ { exact hand Δ p q _ _ ih₁ ih₂ },
+    case all : m Δ p _ ih { exact hall Δ p _ ih },
+    case ex : m Δ t p _ ih { exact hex Δ t p _ ih }
+  end }
+
+protected lemma weakening (h : ⊢ᵀ Δ) : ∀ {Γ}, Δ ⊆ Γ → ⊢ᵀ Γ :=
 begin
-  induction h generalizing Δ p c,
-  case all : m Δ q _ IH
-  { intros eq,
-    have := IH (finset_mlift Δ), }
+  apply rec_on h,
+  { intros m Δ k r v h hneg Γ ss, refine AxL r v (ss h) (ss hneg) },
+  { intros m Δ h Γ ss, refine verum (ss h) },
+  { intros m Δ p q h IH Γ ss,
+    have : ⊢ᵀ insert p Γ, from IH (finset.insert_subset_insert _ (finset.insert_subset.mp ss).2),
+    have : ⊢ᵀ insert (p ⊔ q) Γ, from or_left p q this,
+    refine derivable.cast this (by { simp, exact (finset.insert_subset.mp ss).1}) },
+  { intros m Δ p q h IH Γ ss,
+    have : ⊢ᵀ insert q Γ, from IH (finset.insert_subset_insert _ (finset.insert_subset.mp ss).2),
+    have : ⊢ᵀ insert (p ⊔ q) Γ, from or_right p q this,
+    refine derivable.cast this (by { simp, exact (finset.insert_subset.mp ss).1}) },
+  { intros m Δ p q h₁ h₂ IH₁ IH₂ Γ ss,
+    have l₁ : ⊢ᵀ insert p Γ, from IH₁ (finset.insert_subset_insert _ $ (finset.insert_subset.mp ss).2),
+    have l₂ : ⊢ᵀ insert q Γ, from IH₂ (finset.insert_subset_insert _ $ (finset.insert_subset.mp ss).2),
+    have : ⊢ᵀ insert (p ⊓ q) Γ, from and p q l₁ l₂,
+    refine derivable.cast this (by { simp, exact (finset.insert_subset.mp ss).1}) },
+  { intros m Δ p h IH Γ ss,
+    have : ⊢ᵀ insert p.push (finset_mlift Γ),
+      from IH (finset.insert_subset_insert _ $ finset.image_subset_image (finset.insert_subset.mp ss).2),
+    have : ⊢ᵀ insert (∀'p) Γ := all p this,
+    refine derivable.cast this (by { simp, exact (finset.insert_subset.mp ss).1}) },
+  { intros m Δ t p h IH Γ ss,
+    have : ⊢ᵀ insert (subst t p) Γ, from IH (finset.insert_subset_insert _ (finset.insert_subset.mp ss).2),
+    have : ⊢ᵀ insert (∃'p) Γ := ex t p this,
+    refine derivable.cast this (by { simp, exact (finset.insert_subset.mp ss).1}) }
 end
 
-#check @derivative
-/--/
+end derivable
 
+section
+variables {Δ : finset (formula L m)}
+open axiomatic_classical_logic' axiomatic_classical_logic
 
-lemma provable_of_derivative : ⊢ᵀ Δ → ∅ ⊢ (Δ.image to_fol).disjunction := λ h,
+lemma provable_of_derivative : derivative Δ → ∅ ⊢ (Δ.image to_fol).disjunction := λ h,
 begin
   induction h,
   case AxL : m Δ k r v h nh
@@ -131,63 +197,248 @@ begin
   sorry
 end
 
-def is_terminal {m} (Δ : list (subformula L m 0)) : Prop := ∃ {k} (r : L.pr k) (v), relation r v ∈ Δ ∧ neg_relation r v ∈ Δ
+end
 
-variables (L) [∀ m, encodable (subformula L m 0)] [∀ m, encodable (subterm L m 0)] (M : list (subformula L m 0))
+section search_tree
+
+def is_terminal (Δ : list (subformula L m 0)) : Prop := ∃ {k} (r : L.pr k) (v), relation r v ∈ Δ ∧ neg_relation r v ∈ Δ
+
+variables {L} [∀ k, encodable (L.fn k)] [∀ k, encodable (L.pr k)]
 open encodable
 
-structure search_tree_label :=
-(metavar : ℕ)
-(p_imdex : ℕ)
-(t_index : ℕ)
-(formulae : list (subformula L metavar 0))
-
-inductive search_tree : Type
-| rel : ∀ (Δ : list (subformula L m 0)), ¬is_terminal Δ →
-    search_tree
-
 def decomp : ℕ → list (subformula L m 0) →
-  ℕ × (list (subformula L m 0) ⊕ (list (subformula L m 0) × list (subformula L m 0)) ⊕ list (subformula L (m + 1) 0))
-| s (relation r v :: σ) := ⟨s, sum.inl $ σ ++ [relation r v]⟩
-| s (p ⊓ q :: σ)        := ⟨s, sum.inr $ sum.inl ⟨σ ++ [p], σ ++ [q]⟩⟩
+  set (ℕ × Σ m, list (subformula L m 0))
+| s []                      := { ⟨s, m, []⟩}
+| s (relation r v :: Γ)     := { ⟨s, m, Γ ++ [relation r v]⟩, }
+| s (neg_relation r v :: Γ) := { ⟨s, m, Γ ++ [neg_relation r v]⟩, }
+| s (⊤ :: Γ)                := ∅
+| s (⊥ :: Γ)                := { ⟨s, m, Γ ++ [⊥]⟩, }
+| s (p ⊓ q :: Γ)            := { ⟨s, m, Γ ++ [p]⟩, ⟨s, _, Γ ++ [q]⟩, }
+| s (p ⊔ q :: Γ)            := { ⟨s, m, Γ ++ [p, q]⟩, }
+| s ((fal p) :: Γ)          := { ⟨s, m + 1, Γ.map mlift ++ [push p]⟩, }
+| s ((ex p) :: Γ)           := { ⟨s + 1, m, Γ ++ (option.map (λ t, subst t p) $ fol.subterm.of_nat  L m 0 s).to_list ++ [∃'p]⟩, }
 
 variables {L}
 
-noncomputable def neg_formulae_index (M : set (subformula L m 0)) (i : ℕ) := (option.map subformula.not $ option.filter M $ decode (subformula L m 0) i)
+@[reducible] def search_label (L : language) := ℕ × ℕ × Σ m, list (subformula L m 0)
 
-inductive search_tree_aux (M : set (subformula L m 0)) :
-  ℕ × ℕ × list (subformula L m 0) → ℕ × ℕ × list (subformula L m 0) → Prop
-| rel : ∀ {i j} (σ : list (subformula L m 0)) {k} (r : L.pr k) (v),
-    ¬is_terminal (relation r v :: σ) →    
-    search_tree_aux ⟨i + 1, j, σ ++ [relation r v] ++ (neg_formulae_index M i).to_list⟩
-                    ⟨i,     j, relation r v :: σ⟩
-| and_left : ∀ {i j} (σ : list (subformula L m 0)) (p q : subformula L m 0),
-    ¬is_terminal σ → search_tree_aux ⟨i + 1, j, σ ++ [p] ++ (neg_formulae_index M i).to_list⟩ ⟨i, j, p ⊓ q :: σ⟩ 
-| and_right : ∀ {i j} (σ : list (subformula L m 0)) (p q : subformula L m 0),
-    ¬is_terminal σ → search_tree_aux ⟨i + 1, j, σ ++ [q] ++ (neg_formulae_index M i).to_list⟩ ⟨i, j, p ⊓ q :: σ⟩ 
-| or : ∀ {i j} (σ : list (subformula L m 0)) (p q : subformula L m 0),
-    ¬is_terminal σ → search_tree_aux ⟨i + 1, j, σ ++ [p, q] ++ (neg_formulae_index M i).to_list⟩ ⟨i, j, p ⊔ q :: σ⟩
-| ex : ∀ {i j} (σ : list (subformula L m 0)) (p : subformula L m 1),
-    ¬is_terminal σ →
-    search_tree_aux ⟨i + 1, j + 1, σ ++ [∃'p] ++
-                      (option.map (λ t, subst t p) $ decode (subterm L m 0) j).to_list ++ (neg_formulae_index M i).to_list⟩
-                    ⟨i, j, (∃'p) :: σ⟩ 
+noncomputable def index_of_set (M : set (sentence L)) (i : ℕ) : option (formula L m) :=
+(option.guard (λ i, i ∈ to_nat '' M) i).bind (subformula.of_nat L m 0)
 
-inductive search_tree_aux_gen (M : set (subformula L (m + 1) 0)) :
-  ℕ × ℕ × list (subformula L (m + 1) 0) → ℕ × ℕ × list (subformula L m 0) → Prop
-| univ : ∀ {i j} (σ : list (subformula L m 0)) (p : subformula L m 1),
-    ¬is_terminal σ → search_tree_aux_gen (i, j, σ.map mlift ++ [push p] ++ (neg_formulae_index M i).to_list) (i, j, (∀'p) :: σ)
-
-def search_tree_aux' :  Π {m₁ m₂}, ℕ × ℕ × list (subformula L m₁ 0) → ℕ × ℕ × list (subformula L m₂ 0) → Prop
-| 
-
-lemma nuigigi (M : set (subformula L m 0)) {x} {i j} (σ : list (subformula L m 0)) (p : subformula L m 1) : 
-  search_tree_aux M x ⟨i, j+2, (∃'p) :: σ⟩ → false := λ h,
+@[simp] lemma mlift_index_of_set (M : set (sentence L)) (i : ℕ) :
+  (index_of_set M i : option (formula L m)).map mlift = index_of_set M i :=
 begin
-  cases h, simp[←nat.succ_add] at h,
+  ext p, simp[index_of_set], split,
+  { rintros ⟨q, ⟨i, ⟨rfl, σ, hσ, rfl⟩, h⟩, rfl⟩,
+    refine ⟨σ.to_nat, ⟨rfl, σ, hσ, rfl⟩, _⟩,
+    refine of_nat_eq_some.mpr (by simpa using subformula.of_nat_eq_some.mp h) },
+  { rintros ⟨i, ⟨rfl, σ, hσ, rfl⟩, h⟩,
+    let p' : formula L m := σ.to_uniform.to_subformula (le_trans (subformula_uvars σ) (by simp)),
+    have hp' : to_nat p' = σ.to_nat, by simp[p', to_nat],
+    refine ⟨p', ⟨σ.to_nat, ⟨rfl, σ, hσ, rfl⟩, of_nat_eq_some.mpr hp'⟩, _⟩,
+    refine to_nat_inj.mp (by { simp, symmetry, refine of_nat_eq_some.mp (by simpa[hp'] using h) }) }
 end
+
+lemma index_of_neg_set_eq_some {M : set (sentence L)} {i : ℕ} {p : formula L m} :
+  index_of_set M i = some p → ∃ σ ∈ M, to_nat σ = to_nat p := λ h,
+by { simp[index_of_set] at h, rcases h with ⟨_, ⟨rfl, σ, hσ, rfl⟩, h⟩, 
+     refine ⟨σ, hσ, (subformula.of_nat_eq_some.mp h).symm⟩ } 
+
+@[simp] noncomputable def indices_of_neg_set (M : set (sentence L)) (m) : ℕ → list (formula L m)
+| 0       := []
+| (i + 1) := (index_of_set M i).to_list ++ indices_of_neg_set i
+
+inductive search_tree (M : set (sentence L)) : search_label L → search_label L → Prop
+| intro : ∀ {m₁ m₂} (Γ₁ : list (subformula L m₁ 0)) (Γ₂ : list (subformula L m₂ 0)) (s₁ s₂ i : ℕ),
+    ¬is_terminal Γ₁ → 
+    (s₂, sigma.mk m₂ Γ₂) ∈ decomp s₁ Γ₁ →
+    search_tree ⟨i + 1, s₂, m₂, Γ₂ ++ (index_of_set M i).to_list⟩ ⟨i, s₁, m₁, Γ₁⟩
+
+notation l₁ ` ≺[` :50 M `] ` l₂ :50 := search_tree M l₁ l₂
+
+variables {M : set (sentence L)} {Δ : list (sentence L)}
+
+variables (M Δ)
+
+inductive accessible (Δ : list (sentence L)) : search_label L → Prop
+| top : accessible ⟨0, 0, sigma.mk 0 Δ⟩
+| lt : ∀ {l₁ l₂}, l₁ ≺[M] l₂ → accessible l₂ → accessible l₁
+
+def accessible_label := { l // accessible M Δ l }
+
+def accessible_search_tree : accessible_label M Δ → accessible_label M Δ → Prop :=
+λ l₁ l₂, l₁.val ≺[M] l₂.val 
+
+local infix ` ≺ `:50 := accessible_search_tree M Δ
+
+@[simp] lemma Axl_bot (l) (Γ : list (formula L m)) (h : is_terminal Γ) {i s} : ¬search_tree M l ⟨i, s, _, Γ⟩ :=
+by rintros ⟨⟩; contradiction
+
+section well_founded
+variables {M Δ} (H : well_founded (accessible_search_tree M Δ))
+
+def accessible_search_tree.recursion {C : accessible_label M Δ → Sort*} 
+  (l) (h : Π l₁, (Π l₂, l₂ ≺ l₁ → C l₂) → C l₁) : C l :=
+well_founded.recursion H l h
+
+lemma search_tree_nil (i s) {m} :
+  ⟨i + 1, s, m, (index_of_set M i).to_list⟩ ≺[M] ⟨i, s, m, []⟩ := 
+by { refine search_tree.intro [] [] s s i _ (by simp[decomp]), { simp[is_terminal] } }
+
+lemma search_tree_falsum (i s) {m} (Γ : list (formula L m)) (h : ¬is_terminal (⊥ :: Γ)) :
+  ⟨i + 1, s, m, Γ ++ [⊥] ++ (index_of_set M i).to_list⟩ ≺[M] ⟨i, s, m, ⊥ :: Γ⟩ := 
+search_tree.intro _ _ _ _ _ h (by simp[decomp])
+
+lemma search_tree_relation (i s) {m} (Γ : list (formula L m)) {k} (r : L.pr k) (v : fin k → subterm L m 0)
+  (h : ¬is_terminal (relation r v :: Γ)) :
+  ⟨i + 1, s, m, Γ ++ [relation r v] ++ (index_of_set M i).to_list⟩ ≺[M] ⟨i, s, m, relation r v :: Γ⟩ := 
+search_tree.intro _ _ _ _ _ h (by simp[decomp])
+
+lemma search_tree_neg_relation (i s) {m} (Γ : list (formula L m)) {k} (r : L.pr k) (v : fin k → subterm L m 0)
+  (h : ¬is_terminal (neg_relation r v :: Γ)) :
+  ⟨i + 1, s, m, Γ ++ [neg_relation r v] ++ (index_of_set M i).to_list⟩ ≺[M] ⟨i, s, m, neg_relation r v :: Γ⟩ := 
+search_tree.intro _ _ _ _ _ h (by simp[decomp])
+
+lemma search_tree_and_left (i s) {m} (Γ : list (formula L m)) (p q : formula L m)
+  (h : ¬is_terminal (p ⊓ q :: Γ)) :
+  ⟨i + 1, s, m, Γ ++ [p] ++ (index_of_set M i).to_list⟩ ≺[M] ⟨i, s, m, p ⊓ q :: Γ⟩ := 
+search_tree.intro _ _ _ _ _ h (by simp[decomp])
+
+lemma search_tree_and_right (i s) {m} (Γ : list (formula L m)) (p q : formula L m)
+  (h : ¬is_terminal (p ⊓ q :: Γ)) :
+  ⟨i + 1, s, m, Γ ++ [q] ++ (index_of_set M i).to_list⟩ ≺[M] ⟨i, s, m, p ⊓ q :: Γ⟩ := 
+search_tree.intro _ _ _ _ _ h (by simp[decomp])
+
+lemma search_tree_or (i s) {m} (Γ : list (formula L m)) (p q : formula L m)
+  (h : ¬is_terminal (p ⊔ q :: Γ)) :
+  ⟨i + 1, s, m, Γ ++ [p, q] ++ (index_of_set M i).to_list⟩ ≺[M] ⟨i, s, m, p ⊔ q :: Γ⟩ := 
+search_tree.intro _ _ _ _ _ h (by simp[decomp])
+
+lemma search_tree_fal (i s) {m} (Γ : list (formula L m)) (p : subformula L m 1)
+  (h : ¬is_terminal ((∀'p) :: Γ)) :
+  ⟨i + 1, s, m + 1, Γ.map mlift ++ [p.push] ++ (index_of_set M i).to_list⟩ ≺[M] ⟨i, s, m, (∀'p) :: Γ⟩ := 
+search_tree.intro _ _ _ _ _ h (by simp[decomp, ←fal_eq])
+
+lemma search_tree_ex (i s) {m} (Γ : list (formula L m)) (p : subformula L m 1)
+  (h : ¬is_terminal ((∃'p) :: Γ)) :
+  ⟨i + 1, s + 1, m, Γ ++ (option.map (λ t, subst t p) $ fol.subterm.of_nat L m 0 s).to_list ++
+    [∃'p] ++ (index_of_set M i).to_list⟩ ≺[M] ⟨i, s, m, (∃'p) :: Γ⟩ := 
+search_tree.intro ((∃'p) :: Γ)
+  (Γ ++ (option.map (λ t, subst t p) $ fol.subterm.of_nat L m 0 s).to_list ++ [∃'p]) 
+  s (s + 1) i h (by simp[decomp, ←ex_eq])
+
+
+private lemma synthetic_main_lemma_aux_and {Γ : list (formula L m)} {p q : formula L m} {i} {I₁ I₂ : list ℕ}
+  (d₁ : ⊢ᵀ (Γ ++ [p] ++ (index_of_set M i).to_list).to_finset ∪ (I₁.bind (λ i, (index_of_set M i).to_list)).to_finset)
+  (d₂ : ⊢ᵀ (Γ ++ [q] ++ (index_of_set M i).to_list).to_finset ∪ (I₂.bind (λ i, (index_of_set M i).to_list)).to_finset) : 
+  ⊢ᵀ (p ⊓ q :: Γ).to_finset ∪ ((i :: I₁ ++ I₂).bind (λ i, (index_of_set M i).to_list)).to_finset :=
+begin
+simp at d₁,
+  have d₁ : ⊢ᵀ insert p (Γ.to_finset ∪ ((index_of_set M i).to_finset ∪ ((i :: I₁ ++ I₂).bind (λ i, (index_of_set M i).to_list)).to_finset)),
+    from derivable.weakening d₁ (by intros p; simp[-list.mem_map, -list.mem_bind]; tauto),
+  have d₂ : ⊢ᵀ insert q (Γ.to_finset ∪ ((index_of_set M i).to_finset ∪ ((i :: I₁ ++ I₂).bind (λ i, (index_of_set M i).to_list)).to_finset)),
+    from derivable.weakening d₂ (by intros p; simp[-list.mem_map, -list.mem_bind]; tauto),
+  have : ⊢ᵀ insert (p ⊓ q) (Γ.to_finset ∪ ((index_of_set M i).to_finset ∪ ((i :: I₁ ++ I₂).bind (λ i, (index_of_set M i).to_list)).to_finset)),
+    from derivable.and p q d₁ d₂,
+  exact derivable.cast this (by ext; simp[and_eq])
+end
+
+private lemma synthetic_main_lemma_aux_or {Γ : list (formula L m)} {p q : formula L m} {i} {I : list ℕ}
+  (d : ⊢ᵀ (Γ ++ [p, q] ++ (index_of_set M i).to_list).to_finset ∪ (I.bind (λ i, (index_of_set M i).to_list)).to_finset) : 
+  ⊢ᵀ (p ⊔ q :: Γ).to_finset ∪ ((i :: I).bind (λ i, (index_of_set M i).to_list)).to_finset :=
+begin
+  have : ⊢ᵀ (insert p $ insert q $ Γ.to_finset ∪ ((i :: I).bind (λ i, (index_of_set M i).to_list)).to_finset),
+  by simpa using d,
+  have : ⊢ᵀ (insert q $ insert (p ⊔ q) $ Γ.to_finset ∪ ((i :: I).bind (λ i, (index_of_set M i).to_list)).to_finset),
+    from derivable.cast (derivable.or_left p q this) (finset.insert.comm _ _ _),
+  have : ⊢ᵀ (insert (p ⊔ q) $ Γ.to_finset ∪ ((i :: I).bind (λ i, (index_of_set M i).to_list)).to_finset),
+  from derivable.cast (derivable.or_right p q this) (finset.insert_idem _ _),
+  exact derivable.cast this (by ext x; simp[-list.mem_map, -list.mem_bind])
+end
+
+private lemma synthetic_main_lemma_aux_all {Γ : list (formula L m)} {p : subformula L m 1} {i} {I : list ℕ}
+  (d : ⊢ᵀ (Γ.map mlift ++ [p.push] ++ (index_of_set M i).to_list).to_finset ∪ (I.bind (λ i, (index_of_set M i).to_list)).to_finset) : 
+  ⊢ᵀ ((∀'p) :: Γ).to_finset ∪ ((i :: I).bind (λ i, (index_of_set M i).to_list)).to_finset :=
+begin
+  have : ⊢ᵀ insert p.push (finset_mlift $ Γ.to_finset ∪ ((i :: I).bind (λ i, (index_of_set M i).to_list)).to_finset),
+  { refine derivable.cast d (by { ext p,
+    simp[-list.mem_map, -list.mem_bind, -finset.mem_image, finset_mlift, finset.image_union, 
+      finset.image_to_finset_list, finset.image_to_finset_option, list.bind_map, list.map_to_list_option] }) },
+  have : ⊢ᵀ insert (∀'p) (Γ.to_finset ∪ ((i :: I).bind (λ i, (index_of_set M i).to_list)).to_finset),
+    from derivable.all p this,
+  exact derivable.cast this (by ext x; simp)
+end
+
+private lemma synthetic_main_lemma_aux_ex {Γ : list (formula L m)} {p : subformula L m 1} {i s} {I : list ℕ}
+  (d : ⊢ᵀ (Γ ++ ((subterm.of_nat L m 0 s).map (λ t, subst t p)).to_list ++ [(∃'p : subformula _ _ _)] ++
+    (index_of_set M i).to_list).to_finset ∪ (I.bind (λ i, (index_of_set M i).to_list)).to_finset) : 
+  ⊢ᵀ ((∃'p) :: Γ).to_finset ∪ ((i :: I).bind (λ i, (index_of_set M i).to_list)).to_finset :=
+begin
+  simp at d,
+  cases subterm.of_nat L m 0 s with t; simp at d,
+  { exact derivable.cast d (by ext x; simp) },
+  { have : ⊢ᵀ (insert (subst t p) $ insert (∃'p) $ Γ.to_finset ∪ ((i :: I).bind (λ i, (index_of_set M i).to_list)).to_finset),
+    exact derivable.cast d (by ext; simp[-list.mem_map, -list.mem_bind]; tauto),
+    have : ⊢ᵀ (insert (∃'p) $ Γ.to_finset ∪ ((i :: I).bind (λ i, (index_of_set M i).to_list)).to_finset),
+    exact derivable.cast (derivable.ex t p this) (by ext; simp),
+    exact derivable.cast this (by ext; simp) }
+end
+
+include H
+
+lemma synthetic_main_lemma_aux (l : accessible_label M Δ) : ∃ I : list ℕ,
+  ⊢ᵀ l.val.2.2.2.to_finset ∪ list.to_finset (I.bind (λ i, (index_of_set M i).to_list)) :=
+begin
+  apply accessible_search_tree.recursion H l,
+  rintros ⟨⟨i, s, m, Γ⟩, accΓ⟩ IH,
+  have IH : ∀ (i₂ s₂) {m₂} (Γ₂ : list (subformula L m₂ 0)),
+    ⟨i₂, s₂, m₂, Γ₂⟩ ≺[M] ⟨i, s, m, Γ⟩ →
+    ∃ I : list ℕ, ⊢ᵀ Γ₂.to_finset ∪ list.to_finset (I.bind (λ i, (index_of_set M i).to_list)),
+  { intros i₂ s₂ m₂ Γ₂ h, 
+    have : accessible M Δ ⟨i₂, s₂, m₂, Γ₂⟩, from accessible.lt h accΓ,
+    simpa using IH ⟨⟨i₂, s₂, _, Γ₂⟩, this⟩ h },
+  show ∃ (I : list ℕ), ⊢ᵀ Γ.to_finset ∪ (I.bind (λ i, (index_of_set M i).to_list)).to_finset,
+  by_cases hΓ : is_terminal Γ,
+  { rcases hΓ with ⟨k, r, v, hΓ, hΓ_neg⟩,
+    refine ⟨[], by simp; exact derivable.AxL r v (by simp; refine hΓ) (by simp; refine hΓ_neg)⟩ },
+  cases Γ with p Γ,
+  { rcases IH _ _ _ (search_tree_nil _ _) with ⟨I, d⟩,
+    refine ⟨i :: I, derivable.cast d (by ext; simp)⟩ },
+  cases p,
+  case verum { refine ⟨[], derivable.verum (by simp[verum_eq])⟩ },
+  case falsum
+  { rcases IH _ _ _ (search_tree_falsum _ _ _ hΓ) with ⟨I, d⟩,
+    refine ⟨i :: I, derivable.cast d (by ext; simp[falsum_eq])⟩ },  
+  case relation : k r v
+  { rcases IH _ _ _ (search_tree_relation _ _ _ r v hΓ) with ⟨I, d⟩,
+    refine ⟨i :: I, derivable.cast d (by ext; simp)⟩ },
+  case neg_relation : k r v
+  { rcases IH _ _ _ (search_tree_neg_relation _ _ _ r v hΓ) with ⟨I, d⟩,
+    refine ⟨i :: I, derivable.cast d (by ext; simp)⟩ },
+  case and : p q
+  { rcases IH _ _ _ (search_tree_and_left _ _ _ p q hΓ) with ⟨I₁, d₁⟩,
+    rcases IH _ _ _ (search_tree_and_right _ _ _ p q hΓ) with ⟨I₂, d₂⟩,
+    refine ⟨i :: I₁ ++ I₂, synthetic_main_lemma_aux_and d₁ d₂⟩ },      
+  case or : p q
+  { rcases IH _ _ _ (search_tree_or _ _ _ p q hΓ) with ⟨I, d⟩,
+    refine ⟨i :: I, synthetic_main_lemma_aux_or d⟩ },  
+  case fal : p
+  { rcases IH _ _ _ (search_tree_fal _ _ _ p hΓ) with ⟨I, d⟩,
+    refine ⟨i :: I, synthetic_main_lemma_aux_all d⟩ },
+  case ex : p
+  { rcases IH _ _ _ (search_tree_ex _ _ _ p hΓ) with ⟨I, d⟩,
+    refine ⟨i :: I, synthetic_main_lemma_aux_ex d⟩ }
+end
+
+lemma synthetic_main_lemma (Γ : list (subformula L m 0)) {i s}
+  (h : accessible M Δ ⟨i, s, _, Γ⟩) : 
+  ∃ (I : list ℕ), ⊢ᵀ Γ.to_finset ∪ (I.bind (λ i, (index_of_set M i).to_list)).to_finset :=
+by simpa using synthetic_main_lemma_aux H ⟨_, h⟩
+
+end well_founded
+
+end search_tree
+
 end Tait
-
-
 
 end fol
