src/QL/FOL/Tait/coding.lean
@@ -1,4 +1,4 @@
-import QL.FOL.Tait.tait provability consistency
+import QL.FOL.Tait.tait provability QL.FOL.coding consistency
 
 universes u v
 
@@ -7,51 +7,180 @@ open_locale logic_symbol
 variables {L : language.{u}} {m n : ℕ}
 
 namespace Tait
+variables (L)
 
-namespace subformula
+inductive uniform_subformula : ℕ → Type u
+| verum        {n} : uniform_subformula n
+| falsum       {n} : uniform_subformula n
+| relation     {n} : ∀ {p}, L.pr p → (fin p → uniform_subterm L n) → uniform_subformula n
+| neg_relation {n} : ∀ {p}, L.pr p → (fin p → uniform_subterm L n) → uniform_subformula n
+| and          {n} : uniform_subformula n → uniform_subformula n → uniform_subformula n
+| or           {n} : uniform_subformula n → uniform_subformula n → uniform_subformula n
+| fal          {n} : uniform_subformula (n + 1) → uniform_subformula n
+| ex           {n} : uniform_subformula (n + 1) → uniform_subformula n
+
+namespace uniform_subformula
+variables {L n}
+
+@[simp] def uvars : Π {n}, Tait.uniform_subformula L n → ℕ
+| n verum              := 0
+| n falsum             := 0
+| n (relation r v)     := ⨆ᶠ i, (v i).uvars
+| n (neg_relation r v) := ⨆ᶠ i, (v i).uvars
+| n (and p q)          := max p.uvars q.uvars
+| n (or p q)           := max p.uvars q.uvars
+| n (fal p)            := p.uvars
+| n (ex p)             := p.uvars
+
+@[simp] def to_subformula : ∀ {n} (p : uniform_subformula L n), p.uvars ≤ m → subformula L m n
+| n verum              h := ⊤
+| n falsum             h := ⊥
+| n (relation r v)     h := subformula.relation r (λ i, (v i).to_subterm (by show (v i).uvars ≤ m; simp at h; exact h i))
+| n (neg_relation r v) h := subformula.neg_relation r (λ i, (v i).to_subterm (by show (v i).uvars ≤ m; simp at h; exact h i))
+| n (and p q)          h := have h : p.uvars ≤ m ∧ q.uvars ≤ m, by simpa using h, p.to_subformula h.1 ⊓ q.to_subformula h.2
+| n (or p q)           h := have h : p.uvars ≤ m ∧ q.uvars ≤ m, by simpa using h, p.to_subformula h.1 ⊔ q.to_subformula h.2
+| n (fal p)            h := ∀'p.to_subformula (by simpa using h)
+| n (ex p)             h := ∃'p.to_subformula (by simpa using h)
 
 section encode
+open encodable nat
+variables {L n} [∀ k, encodable (L.pr k)] [∀ k, encodable (L.fn k)]
+
+@[simp] def to_nat : Π {n}, uniform_subformula L n → ℕ
+| n verum                     := 0
+| n falsum                    := 1
+| n (@relation L _ k r v)     := (bit0 $ bit0 $ mkpair k $ mkpair (encode r) (encode v)) + 2
+| n (@neg_relation L _ k r v) := (bit0 $ bit1 $ mkpair k $ mkpair (encode r) (encode v)) + 2
+| n (and p q)                 := (bit1 $ bit0 $ bit0 $ mkpair p.to_nat q.to_nat) + 2
+| n (or p q)                  := (bit1 $ bit0 $ bit1 $ mkpair p.to_nat q.to_nat) + 2
+| n (fal p)                   := (bit1 $ bit1 $ bit0 p.to_nat) + 2
+| n (ex p)                    := (bit1 $ bit1 $ bit1 p.to_nat) + 2
+
+variables (L n)
+
+@[simp] def of_nat : Π n, ℕ → option (uniform_subformula L n)
+| n 0 := some verum
+| n 1 := some falsum
+| n (e + 2) :=
+    let i := e.div2.div2.div2 in
+    have div8 : i ≤ e := by simp[i, nat.div2_val]; 
+      exact le_trans (nat.div_le_self (e / 2 / 2) 2) (le_trans (nat.div_le_self (e/2) 2) (nat.div_le_self e 2)),
+    have hi : i < e + 2, from lt.step (lt_succ_iff.mpr div8),
+    have hi1 : i.unpair.1 < e + 2, from (lt.step $ nat.lt_succ_iff.mpr (le_trans (nat.unpair_left_le _) div8)),
+    have hi2 : i.unpair.2 < e + 2, from (lt.step $ nat.lt_succ_iff.mpr (le_trans (nat.unpair_right_le _) div8)),
+    match e.bodd with
+    | ff :=
+      match e.div2.bodd with
+      | ff :=
+        let x := e.div2.div2,
+            k := x.unpair.1,
+            r := decode₂ (L.pr k) x.unpair.2.unpair.1,
+            v := decode₂ (fin k → uniform_subterm L n) x.unpair.2.unpair.2 in
+        r.bind (λ r, v.map (relation r))
+      | tt :=
+        let x := e.div2.div2,
+            k := x.unpair.1,
+            r := decode₂ (L.pr k) x.unpair.2.unpair.1,
+            v := decode₂ (fin k → uniform_subterm L n) x.unpair.2.unpair.2 in
+        r.bind (λ r, v.map (neg_relation r))
+      end
+    | tt :=
+      match e.div2.bodd, e.div2.div2.bodd with
+      | ff, ff := (of_nat n i.unpair.1).bind (λ p, (of_nat n i.unpair.2).map (and p))
+      | ff, tt := (of_nat n i.unpair.1).bind (λ p, (of_nat n i.unpair.2).map (or p))
+      | tt, ff := (of_nat (n + 1) i).map fal
+      | tt, tt := (of_nat (n + 1) i).map ex
+      end
+    end
+using_well_founded {rel_tac := λ _ _, `[exact ⟨_, measure_wf (λ x, x.2)⟩]}
+
+@[simp] lemma of_nat_to_nat : ∀ {n} (p : uniform_subformula L n), of_nat L n p.to_nat = some p
+| n verum                     := by simp
+| n falsum                    := by simp
+| n (@relation L _ k r v)     :=
+    begin
+      simp only [to_nat, of_nat, nat.bodd_bit0, nat.div2_bit0, nat.unpair_mkpair],
+      rw[show (unpair (bit0 (bit0 (mkpair k (mkpair (encode r) (encode v))))).div2.div2).fst = k, by simp],
+      simp only [decode₂_encode, option.some_bind', option.map_some', heq.refl], simp
+    end
+| n (@neg_relation L _ k r v) :=
+    begin
+      simp only [to_nat, of_nat, nat.bodd_bit0, nat.bodd_bit1, nat.div2_bit0, nat.div2_bit1, nat.unpair_mkpair],
+      rw[show (unpair (bit0 (bit1 (mkpair k (mkpair (encode r) (encode v))))).div2.div2).fst = k, by simp],
+      simp only [decode₂_encode, option.some_bind', option.map_some', heq.refl], simp
+    end
+| n (and p q)                 := by simp; refine ⟨of_nat_to_nat p, of_nat_to_nat q⟩
+| n (or p q)                  := by simp; refine ⟨of_nat_to_nat p, of_nat_to_nat q⟩
+| n (fal p)                   := by simp; refine (of_nat_to_nat p)
+| n (ex p)                    := by simp; refine (of_nat_to_nat p)
+
+instance (n) : encodable (uniform_subformula L n) :=
+{ encode := to_nat,
+  decode := of_nat L n,
+  encodek := by simp }
+
+end encode
+
+end uniform_subformula
+
+namespace subformula
+open uniform_subformula
+variables {L m n}
+
+@[simp] def to_uniform : Π {n}, subformula L m n → uniform_subformula L n
+| n verum              := uniform_subformula.verum
+| n falsum             := uniform_subformula.falsum
+| n (relation r v)     := uniform_subformula.relation r (subterm.to_uniform ∘ v)
+| n (neg_relation r v) := uniform_subformula.neg_relation r (subterm.to_uniform ∘ v)
+| n (and p q)          := uniform_subformula.and p.to_uniform q.to_uniform
+| n (or p q)           := uniform_subformula.or p.to_uniform q.to_uniform
+| n (fal p)            := uniform_subformula.fal p.to_uniform
+| n (ex p)             := uniform_subformula.ex p.to_uniform
+
+@[simp] lemma to_uniform_mlift (p : subformula L m n) : p.mlift.to_uniform = p.to_uniform :=
+by simp[mlift]; induction p; simp[mlift', ←fal_eq, ←verum_eq, ←falsum_eq, ←and_eq, ←or_eq, ←fal_eq, ←ex_eq, (∘), *]
+
+@[simp] lemma to_uniform_to_subterm (p : subformula L m n) (h) : p.to_uniform.to_subformula h = p :=
+by induction p; simp*; refl
+
+@[simp] lemma to_subterm_to_uniform (p : uniform_subformula L n) (h : p.uvars ≤ m) : (p.to_subformula h).to_uniform = p :=
+by induction p; simp[←fal_eq, ←verum_eq, ←falsum_eq, ←and_eq, ←or_eq, ←fal_eq, ←ex_eq, (∘), *]
+
+section encode
+
+variables [∀ k, encodable (L.fn k)] [∀ k, encodable (L.pr k)]
+
+def to_nat : subformula L m n → ℕ := λ p, encodable.encode p.to_uniform
+
 variables (L m n)
 
-def label :=
-  unit ⊕ unit ⊕
-  (Σ k, L.pr k × (fin k → subterm L m n)) ⊕ (Σ k, L.pr k × (fin k → subterm L m n)) ⊕
-  unit ⊕ unit ⊕
-  unit ⊕ unit
-
-def arity : label L m n → Type
-| (sum.inl _)                                                             := empty
-| (sum.inr $ sum.inl _)                                                   := empty
-| (sum.inr $ sum.inr $ sum.inl _)                                         := empty
-| (sum.inr $ sum.inr $ sum.inr $ sum.inl _)                               := empty
-| (sum.inr $ sum.inr $ sum.inr $ sum.inr $ sum.inl _)                     := bool
-| (sum.inr $ sum.inr $ sum.inr $ sum.inr $ sum.inr $ sum.inl _)           := bool
-| (sum.inr $ sum.inr $ sum.inr $ sum.inr $ sum.inr $ sum.inr $ sum.inl _) := unit
-| (sum.inr $ sum.inr $ sum.inr $ sum.inr $ sum.inr $ sum.inr $ sum.inr _) := unit
+def of_nat : ℕ → option (subformula L m n) := λ i,
+  let p := encodable.decode₂ (uniform_subformula L n) i in
+  p.bind (λ p, if h : p.uvars ≤ m then some (p.to_subformula h) else none)
 
 variables {L m n}
 
-@[reducible] def W_to_subformula : W_type (arity L m n) → subformula L m n
-| ⟨sum.inl x, _⟩                := ⊤
-| ⟨sum.inr $ sum.inl ⟨k, r, v⟩, _⟩ := relation r v
-| ⟨sum.inr $ sum.inr $ sum.inl _, F⟩ := (W_to_subformula (F ff)) ⟶ (W_to_subformula (F tt))
-| ⟨sum.inr $ sum.inr $ sum.inr $ sum.inl _, F⟩ := ∼W_to_subformula (F ())
-| ⟨sum.inr $ sum.inr $ sum.inr $ sum.inr _, F⟩ := by {  }
+@[simp] lemma subformula_uvars (p : subformula L m n) : p.to_uniform.uvars ≤ m :=
+by induction p; simp*
 
-#check Tait.subformula
+@[simp] lemma to_nat_of_nat (p : subformula L m n) : of_nat L m n p.to_nat = some p :=
+by simp[to_nat, of_nat]
 
-def subformula_to_W : (Σ n, subformula L m n) → (Σ n, W_type (arity L m n))
-| ⟨n, verum⟩            := ⟨n, sum.inl (), empty.rec _⟩
-| ⟨n, falsum⟩           := ⟨n, sum.inr $ sum.inl (), empty.rec _⟩
-| ⟨n, relation r v⟩     := ⟨n, sum.inr $ sum.inr $ sum.inl ⟨_, r, v⟩, empty.rec _⟩
-| ⟨n, neg_relation r v⟩ := ⟨n, sum.inr $ sum.inr $ sum.inr $ sum.inl ⟨_, r, v⟩, empty.rec _⟩
-| ⟨n, and p q⟩          := ⟨n, sum.inr $ sum.inr $ sum.inr $ sum.inr $ sum.inl (), λ b, bool.cases_on b (subformula_to_W p) (subformula_to_W q)⟩
-| ⟨n, or p q⟩           := ⟨n, sum.inr $ sum.inr $ sum.inr $ sum.inr $ sum.inr $ sum.inl (), λ b, bool.cases_on b (subformula_to_W p) (subformula_to_W q)⟩
-| ⟨n, fal p⟩            := ⟨n + 1, sum.inr $ sum.inr $ sum.inr $ sum.inr $ sum.inr $ sum.inr $ sum.inl (), λ _, subformula_to_W p⟩
-| ⟨n, ex p⟩             := ⟨n + 1, sum.inr $ sum.inr $ sum.inr $ sum.inr $ sum.inr $ sum.inr $ sum.inr (), λ _, subformula_to_W p⟩
---using_well_founded {rel_tac := λ _ _, `[exact ⟨_, measure_wf (λ x, x.2.complexity)⟩]}
+@[simp] lemma of_nat_to_nat (p : subformula L m n) : to_nat p.mlift = to_nat p :=
+by simp[to_nat]
+
+lemma of_nat_eq_some {e} {p : subformula L m n} : of_nat L m n e = some p ↔ p.to_nat = e :=
+by { simp[of_nat, to_nat, encodable.decode₂_eq_some, dite_eq_iff], split,
+  { simp, rintros _ rfl h rfl, simp },
+  { rintros rfl, refine ⟨p.to_uniform, rfl, by simp⟩ } }
+
+lemma of_nat_eq_som {m₁ m₂} {p : subformula L m₁ n} {q : subformula L m₂ n} : p.to_nat = q.to_nat ↔ p.to_uniform = q.to_uniform :=
+by simp[to_nat]
 
 
+@[simp] lemma to_nat_inj {p q : subformula L m n} : p.to_nat = q.to_nat ↔ p = q :=
+by { have : q = p ↔ p.to_nat = q.to_nat, by simpa using @of_nat_eq_some _ _ _ _ _ q.to_nat p,
+     simp[←this], exact comm }
 
 end encode
 
